src/RIoT.DerEnc.fst
@@ -1,0 +1,192 @@
+module RIoT.DerEnc
+
+open Common
+//open RIoT.Common
+
+open LowStar.BufferOps
+open FStar.Integers
+//open Lib.IntTypes
+
+open Spec.Hash.Definitions
+open Hacl.Hash.Definitions
+
+module I  = FStar.Integers
+module HI  = Lib.IntTypes
+
+module SHA2= Hacl.Hash.SHA2
+module HMAC= Hacl.HMAC
+module Ed25519 = Hacl.Ed25519
+
+module CL  = C.Loops
+module CE  = C.Endianness
+module CF  = C.Failure
+module C   = C
+module CS  = C.String
+module S   = FStar.Seq
+module IB  = LowStar.ImmutableBuffer
+module B   = LowStar.Buffer
+module M   = LowStar.Modifies
+module HS  = FStar.HyperStack
+module HST = FStar.HyperStack.ST
+
+///      //
+///      // Context structure for the DER-encoder. This structure contains a fixed-
+///      // length array for nested SEQUENCES (which imposes a nesting limit).
+///      // The buffer use for encoded data is caller-allocted.
+///      //
+///      typedef struct
+///      {
+///          uint8_t     *Buffer;        // Encoded data
+///          uint32_t     Length;        // Size, in bytes, of Buffer
+///          uint32_t     Position;      // Current buffer position
+///
+///          // SETS, SEQUENCES, etc. can be nested. This array contains the start of
+///          // the payload for collection types and is set by  DERStartSequenceOrSet().
+///          // Collections are "popped" using DEREndSequenceOrSet().
+///          int CollectionStart[DER_MAX_NESTED];
+///          int CollectionPos;
+///      } DERBuilderContext;
+noeq
+type derBuilderContext = {
+     derCtxLength   : uint_32;
+     derCtxBuffer   : B.lbuffer HI.uint8 (v derCtxLength);
+     derCtxPosition : uint_32
+  }
+
+let live_derCtx
+  (h: Monotonic.HyperStack.mem)
+  (ctx: derBuilderContext)
+: GTot Type0
+= B.live h ctx.derCtxBuffer
+
+let disjoint_derCtx
+  (ctx1 ctx2: derBuilderContext)
+: GTot Type0
+= B.disjoint ctx1.derCtxBuffer ctx2.derCtxBuffer
+
+///      // We only have a small subset of potential PEM encodings
+///      enum CertType {
+///          CERT_TYPE = 0,
+///          PUBLICKEY_TYPE,
+///          ECC_PRIVATEKEY_TYPE,
+///          CERT_REQ_TYPE,
+///          LAST_CERT_TYPE
+///      };
+type certType =
+| CERT_TYPE
+| PUBLICKEY_TYPE
+| ECC_PRIVATEKEY_TYPE
+| CERT_REQ_TYPE
+| LAST_CERT_TYPE
+
+
+///
+///      //
+///      // This file contains basic DER-encoding routines that are sufficient to create
+///      // RIoT X.509 certificates. A few corners are cut (and noted) in the interests
+///      // of small code footprint and simplicity.
+///      //
+///      // Routines in this file encode the following types:
+///      //    SEQUENCE
+///      //    SET
+///      //    INTEGER
+///      //    OID
+///      //    BOOL
+///      //    PrintableString
+///      //    UTF8String
+///      //    UTCTime
+///      //
+///
+
+
+///      // Assert-less assert
+///      #define ASRT(_X) if(!(_X)) {goto Error;}
+/// NOTE: I'm going to encode this into an if-then-else statement
+
+
+///      // The encoding routines need to check that the encoded data will fit in the
+///      // buffer. The following macros do (conservative) checks because it's hard to
+///      // properly test low-buffer situations. CHECK_SPACE is appropriate for short
+///      // additions. CHECK_SPACE2 when larger objects are being added (and the length
+///      // is known.)
+///      #define CHECK_SPACE(_X)      if((_X->Length-_X->Position)<32)        {goto Error;}
+open FStar.Error
+let riotResult = optResult int_32 int_32
+
+let check_space
+  (_X: derBuilderContext)
+: HST.Stack bool
+  (requires fun h ->
+      live_derCtx h _X
+    /\ ok I.op_Subtraction _X.derCtxLength _X.derCtxPosition)
+  (ensures  fun h0 _ h1 -> True)
+=
+  (_X.derCtxLength - _X.derCtxPosition) < 32ul
+
+let r: uint_8 = cast (-1l)
+
+/// NOTE: demostrate my current encoding way
+/// REF: static int
+///      EncodeInt(
+///          uint8_t     *Buffer,
+///          int          Val
+///      )
+let encodeInt
+  (b: B.buffer uint_8)
+  (value: uint_32)
+: HST.Stack riotResult
+  (requires fun h ->
+      B.live h b
+    /\ (value < 128ul ->
+          B.length b > 1
+        /\ cast_ok (Unsigned W8) value)
+    /\ ((128ul <= value /\ value < 256ul) ->
+          B.length b > 2
+        /\ cast_ok (Unsigned W8) value)
+    /\ ((256ul <= value /\ value < 166536ul) ->
+          B.length b > 3
+        // /\ ok (/) value 256ul
+        /\ within_bounds (Unsigned W32) ((v value) / 256)
+        // /\ ok (%) value 256ul
+        /\ within_bounds (Unsigned W32) ((v value) % 256)
+        /\ cast_ok (Unsigned W8) value))
+  (ensures fun h0 _ h1 -> True)
+///      // DER-encode Val into buffer. Function assumes the caller knows how many
+///      // bytes it will need (e.g., from GetIntEncodedNumBytes).
+=
+///
+/// REF:     ASRT(Val < 166536);  //Recall: #define ASRT(_X) if(!(_X)) {goto Error;}
+  if value < 166536ul then
+///
+/// REF:     if (Val <128) {
+///              Buffer[0] = (uint8_t)Val;
+///              return 0;
+///          }
+    if value < 128ul then
+      ( b.(0ul) <- cast value
+      ; Correct 0l )
+///
+/// REF:     if (Val < 256) {
+///              Buffer[0] = 0x81;
+///              Buffer[1] = (uint8_t)Val;
+///              return 0;
+///          }
+    else if value < 256ul then
+      ( b.(0ul) <- 0x82uy
+      ; b.(1ul) <- cast value
+      ; Correct 0l )
+///
+/// REF:     Buffer[0] = 0x82;
+///          Buffer[1] = (uint8_t)(Val / 256);
+///          Buffer[2] = Val % 256;
+///          return 0;
+    else
+      ( b.(0ul) <- 0x82uy
+      ; b.(1ul) <- cast (value / 256ul)
+      ; b.(2ul) <- cast (value % 256ul)
+      ; Correct 0l )
+  else
+///
+/// REF: Error:
+///          return -1;
+    Error (-1l)
